\section{Conjuntos}

\begin{lemma}[Leis de De Morgan]
    Se \(A_i \subset X\) então, 
    \[(a)\ X\setminus \bigcup A_i = \bigcap (X \setminus A_i) \ \ \text{ e } \ \ (b) \ X\setminus \bigcap A_i = \bigcup (X\setminus A_i). \]
    \textcolor{gray}{\(\rightarrow\) Faz \((a)\) por double contenção e use ele para concluir \((b)\)}
\end{lemma}

\begin{lemma}[Pre-imagen bém portada]
    Sejam \(f:X\to Y\) função e \(B_i \subset Y\). Então,
    \[(a)\ f^{-1}\left(\bigcup B_i\right) = \bigcup f^{-1}(B_i); \ \ \ (b)\ f^{-1}\left(\bigcap B_i\right) = \bigcap f^{-1}(B_i)\]
    \[(c)\ f^{-1}\left(Y \setminus B_i\right) = X \setminus f^{-1}(B_i)\]
\end{lemma}


